proof/correctness/BitEncoding_hakyber.ec
@@ -1,0 +1,43 @@
+require import AllCore IntDiv Array256 Array128.
+require import List Ring StdOrder Fq.
+require import IntMin.
+require import List_extra Ring_extra RealExp_extra IntDiv_extra.
+require import List_hakyber IntDiv_hakyber For.
+
+import Fq IntOrder.
+
+import Kyber_.
+import ZModField.
+import BitEncoding.BS2Int.
+
+
+  op bitrev (i k : int) = bs2int (rev (int2bs i k)).
+
+  lemma bitrev_ineq (i k : int) :
+    0 <= i =>
+    0 <= bitrev i k < 2 ^ i.
+  proof.
+    move => le0i; split; [apply bs2int_ge0|move => _]; rewrite /bitrev; move: (size_int2bs i k) => @/max.
+    by case: (0 < i) => [_ {2}<-|lei0]; [|(have <-: (i = 0) by smt()); move => {2}<-]; rewrite -size_rev; apply bs2int_le2Xs.
+  qed.
+
+  lemma bitrev_involutive (i k : int) :
+    0 <= i =>
+    k \in range 0 (2 ^ i) =>
+    bitrev i (bitrev i k) = k.
+  proof.
+    move => le0i /mem_range [le0k ltk2powi] @/bitrev.
+    suff {1}->: i = size (rev (int2bs i k)).
+    - by rewrite bs2intK revK int2bsK.
+    by rewrite size_rev size_int2bs ler_maxr.
+  qed.
+
+  lemma bitrev_injective (i k1 k2 : int) :
+    0 <= i =>
+    k1 \in range 0 (2 ^ i) =>
+    k2 \in range 0 (2 ^ i) =>
+    bitrev i k1 = bitrev i k2 =>
+    k1 = k2.
+  proof.
+    by move => le0i Hk1in Hk2in eq_bitrev; rewrite -(bitrev_involutive i k1) // -(bitrev_involutive i k2) // eq_bitrev.
+  qed.
