proof/correctness/List_extra.ec
@@ -1,0 +1,4 @@
+require import AllCore List.
+
+lemma all_predI p1 p2 (s : 'a list): all (predI p1 p2) s = (all p1 s /\ all p2 s).
+proof. by elim: s => //= x s ->; rewrite /predI /=; case: (p1 x); case (p2 x). qed.
